Core/Ty/Structure.lean
@@ -129,4 +129,6 @@ def Ty.is_data (data1 : String) (A : Ty) : Bool :=
   | some (data2, _) => data1 == data2
   | none => false
 
+theorem Ty.mkApps_nats_spine (T : String) (ts : List Nat) : ((gt#T).mkApps_nats ts).spine = some (T, ts.map (t#·)) := by sorry
+
 end Core
