Intermediate/Typing.lean
@@ -71,12 +71,12 @@ inductive GlobalWf : GlobalEnv -> Global -> Prop where
   G&[] ⊢ T : ★ ->
   lookup x G = none ->
   GlobalWf G (.defn ⟨x, T, t⟩)
-| classDecl :
+| classDecl {na : Nat} {Ks1 : Vec Core.Kind na}:
   lookup s G = none ->
   ∀ i j: Nat, (hi : i < mτs.length) -> (hj : j < mτs.length) -> i ≠ j -> (mτs[i]'hi).1 ≠ (mτs[j]'hj).1 ->
   (∀ i : Nat, (hi : i < mτs.length) -> mτs[i]'hi = (mn, ⟨na, Ks1, 0, #(), 1, #(T), R⟩) ->
     mn ≠ s ∧ lookup mn G = none ∧ T.spine = some (s, tys) ∧ tys.length = Ks1.length ∧ G&Ks1.list.reverse ⊢ R : ★) ->
-  GlobalWf G (.classDecl ⟨s, K, [],[], mτs⟩)
+  GlobalWf G (.classDecl ⟨s, na, Ks1, [],[], mτs⟩)
 
 | inst {mτs : List (String × Core.SpineTy)} {mths_impl : List (String × (m : Nat) × Core.Pattern m × Surface.Term)}:
   lookup x G = none ->
